bench/process-results.py
@@ -7,15 +7,14 @@ def parse_file(filepath):
     # open the file and read through it line by line
     with open(filepath, 'r') as f:
         for line in f:
-            contents = line.split(' ')
-            if (contents[0] != "DATA:"):
-              continue
-            
-            num = float(contents[1])
-            sec = float(contents[2])
-            nums.append(num)
-            secs.append(sec)
-            ratios.append((num/sec)*1000000)
+            if ("DATA:" in line):
+                contents = line.split("DATA: ")
+                nums = contents[1].split(" ")        
+                num = float(nums[0])
+                sec = float(nums[1])
+                nums.append(num)
+                secs.append(sec)
+                ratios.append((num/sec)*1000000)
 
     nums_np = np.array(nums)
     secs_np = np.array(secs)
@@ -46,52 +45,10 @@ def parse_file(filepath):
     print("")
 
 if __name__== "__main__":
-    print("=== dfscq/smallfile ===")
-    parse_file("results/dfscq/smallfile")
-
-    print("=== dfscq/createdelete ===")
-    parse_file("results/dfscq/createdelete")
-
-    print("=== dfscq/rename ===")
-    parse_file("results/dfscq/rename")
-
-
-    print("=== db_dfscq/smallfile ===")
-    parse_file("results/db_dfscq/smallfile")
-
-    print("=== db_dfscq/createdelete ===")
-    parse_file("results/db_dfscq/createdelete")
-
-    print("=== db_dfscq/rename ===")
-    parse_file("results/db_dfscq/rename")
-
-
-    print("=== fa_dfscq/smallfile ===")
-    parse_file("results/fa_dfscq/smallfile")
-
-    print("=== fa_dfscq/createdelete ===")
-    parse_file("results/fa_dfscq/createdelete")
-
-    print("=== fa_dfscq/rename ===")
-    parse_file("results/fa_dfscq/rename")
-
-
-    print("=== db_fa_dfscq/smallfile ===")
-    parse_file("results/db_fa_dfscq/smallfile")
-
-    print("=== db_fa_dfscq/createdelete ===")
-    parse_file("results/db_fa_dfscq/createdelete")
-
-    print("=== db_fa_dfscq/rename ===")
-    parse_file("results/db_fa_dfscq/rename")
-
-
-    print("=== sfscq/smallfile ===")
-    parse_file("results/sfscq/smallfile")
-
-    print("=== sfscq/createdelete ===")
-    parse_file("results/sfscq/createdelete")
-
-    print("=== sfscq/rename ===")
-    parse_file("results/sfscq/rename")
+    fs_names = ["ConFs", "Cfscq", "Sfscq"]
+    test_names = ["smallfile", "createdelete", "rename"]
+    for test in test_names:
+        for fs in fs_names:
+            print("===", fs, test, "===")
+            parse_file("results/"+fs+"/"+test)
 
