bench/compile-and-run.sh
@@ -3,7 +3,16 @@ cd ../src/Extraction/
 cd ../../bench
 mv ../src/Extraction/extracted/ConFs ./fs/ConFs
 mv ../src/Extraction/extracted/mkfs ./fs/ConMkfs
+
+cd ../../fscq/fscq15/src/
+make
+cd ../../../ConFrm/bench
+mv ../../fscq/fscq15/src/fuse ./fs/CfscqFs
+mv ../../fscq/fscq15/src/mkfs ./fs/CfscqMkfs
+
 ./compile-sources.sh
-./run-confs.sh 10
-#./run-sfscq.sh 10
-./run-cfscq.sh 10
+./run-confs.sh 10 $1
+#./run-sfscq.sh 10 $1
+#./run-cfscq.sh 10 $1
+
+./get-stats.sh
