bench/run-confs.sh
@@ -1,7 +1,8 @@
 ITER=$1
+DEV=$2
 
-if [ $# -ne 1 ]; then
-  echo "$0 iteration-num"
+if [ $# -ne 2 ]; then
+  echo "$0 iteration-num dev-path"
   exit 1
 fi
 
@@ -12,13 +13,13 @@ mkdir results/ConFs
 echo "=== Running ConFs Tests ==="
 
 echo "== smallfile =="
-./run_script.sh Con smallfile /dev/sdb3 $ITER > results/ConFs/smallfile
+./run_script.sh Con smallfile $DEV $ITER > results/ConFs/smallfile
 echo "== largefile =="
-./run_script.sh Con largefile /dev/sdb3 $ITER > results/ConFs/largefile
+./run_script.sh Con largefile $DEV $ITER > results/ConFs/largefile
 echo "== createdelete =="
-./run_script.sh Con createdelete /dev/sdb3 $ITER > results/ConFs/createdelete
+./run_script.sh Con createdelete $DEV $ITER > results/ConFs/createdelete
 echo "== rename =="
-./run_script.sh Con rename /dev/sdb3 $ITER > results/ConFs/rename
+./run_script.sh Con rename $DEV $ITER > results/ConFs/rename
 
 #python process-results.py > results.txt
 #python process-results-largefile.py >> results.txt
