bench/run-sfscq.sh
@@ -1,7 +1,8 @@
 ITER=$1
+DEV=$2
 
-if [ $# -ne 1 ]; then
-  echo "$0 iteration-num"
+if [ $# -ne 2 ]; then
+  echo "$0 iteration-num dev-path"
   exit 1
 fi
 
@@ -12,10 +13,10 @@ mkdir results/Sfscq
 echo "=== Running Sfscq Tests ==="
 
 echo "== smallfile =="
-./run_script.sh Sfscq smallfile /dev/sdb3 $ITER > results/Sfscq/smallfile
+./run_script.sh Sfscq smallfile $DEV $ITER > results/Sfscq/smallfile
 echo "== largefile =="
-./run_script.sh Sfscq largefile /dev/sdb3 $ITER > results/Sfscq/largefile
+./run_script.sh Sfscq largefile $DEV $ITER > results/Sfscq/largefile
 echo "== createdelete =="
-./run_script.sh Sfscq createdelete /dev/sdb3 $ITER > results/Sfscq/createdelete
+./run_script.sh Sfscq createdelete $DEV $ITER > results/Sfscq/createdelete
 echo "== rename =="
-./run_script.sh Sfscq rename /dev/sdb3 $ITER > results/Sfscq/rename
+./run_script.sh Sfscq rename $DEV $ITER > results/Sfscq/rename
